#### 3-3
(1) $\overline{F}=\overline{A}·\overline{\overline{B}·C·\overline{\overline{D}·E}}$

(2) $\overline{F}=\overline{B}+[(\overline{C}+D)·\overline{A}·E]$

(4) $\overline{F}=[(\overline{A}+\overline{B})·(A+B)]+(\overline{C}·\overline{D})+[\overline{E}·(C+D)]$

#### 3-5
(2) 
$$
\begin{cases}
F &= \bar{Y}Z+WX\bar{Y}+WX\bar{Z}+\bar{W}\bar{X}Z \\
  &= \bar{Y}Z(W+\bar{W})(X+\bar{X})+WX\bar{Y}(Z+\bar{Z})+WX\bar{Z}(Y+\bar{Y})+\bar{W}\bar{X}Z(Y+\bar{Y}) \\
  &= \bar{Y}ZWX+\bar{Y}ZW\bar{X}+\bar{Y}Z\bar{W}X+\bar{Y}Z\bar{W}\bar{X}+WX\bar{Y}Z+WX\bar{Y}\bar{Z}+WX\bar{Z}Y+WX\bar{Z}\bar{Y}+\bar{W}\bar{X}ZY+\bar{W}\bar{X}Z\bar{Y} \\
  &= WX\bar{Y}Z+W\bar{X}\bar{Y}Z+\bar{W}X\bar{Y}Z+\bar{W}\bar{X}\bar{Y}Z+WX\bar{Y}\bar{Z}+WXY\bar{Z}+\bar{W}\bar{X}YZ \\
  &=\sum(m_{13}+m_9+m_5+m_1+m_{12}+m_{14}+m_3)

\end{cases}
$$
